src/Manifest_Generator.v
@@ -28,6 +28,12 @@ Fixpoint appr_manifest_update (G : GlobalContext) (e : EvidenceT)
     | None => errC err_str_asp_no_compat_appr_asp
     | Some appr_asp_id => resultC (aspid_manifest_update appr_asp_id m)
     end
+  | left_evt e' => 
+    res <- apply_to_left_evt G (fun e => appr_manifest_update G e m) e' ;;
+    res
+  | right_evt e' => 
+    res <- apply_to_right_evt G (fun e => appr_manifest_update G e m) e' ;;
+    res
   | split_evt e1 e2 => 
     m1 <- appr_manifest_update G e1 m ;;
     appr_manifest_update G e2 m1
